better definition for the abstract clauses

Weidenbach_Book/CDCL_Two_Watched_Literals_Implementation.thy
@@ -43,51 +43,154 @@ text \<open>It is important to remember that a conflicting clause with respect t
 datatype 'v twl_clause =
   TWL_Clause (watched: 'v) (unwatched: 'v)
 
-locale raw_clss_with_update =
-  raw_clss get_lit mset_cls get_cls mset_clss
-  for
-    get_lit :: "'cls \<Rightarrow> 'lit \<Rightarrow> 'v literal option" and
-    mset_cls :: "'cls \<Rightarrow> 'v clause" and
+fun clause :: "'a twl_clause \<Rightarrow> 'a :: {plus}"  where
+"clause (TWL_Clause W UW) = W + UW"
 
-    get_cls :: "'clss \<Rightarrow> 'cls_it \<Rightarrow> 'cls option" and
-    mset_clss:: "'clss \<Rightarrow> 'cls multiset" +
+locale abstract_clause_representation_ops =
   fixes
-    twl_cls :: "'cls \<Rightarrow> 'v literal list twl_clause" and
-    clss_update :: "'clss \<Rightarrow> 'cls_it \<Rightarrow> 'cls \<Rightarrow> 'clss" and
-    swap_lit :: "'cls \<Rightarrow> 'lit \<Rightarrow> 'lit \<Rightarrow> 'cls"
+    lit_lookup :: "'cls \<Rightarrow> 'lit \<Rightarrow> 'v literal option" and
+    lit_keys :: "'cls \<Rightarrow> 'lit multiset" and
+
+    twl_cls :: "'cls \<Rightarrow> 'lit multiset twl_clause" and
+    swap_lit :: "'cls \<Rightarrow> 'lit \<Rightarrow> 'lit \<Rightarrow> 'cls" and
+    it_of_other_watched :: "'cls \<Rightarrow> 'lit \<Rightarrow> 'lit option" and
+    cls_ot_twl_list :: "'v literal list twl_clause \<Rightarrow> 'cls"
+begin
+
+abbreviation twl_clause :: "'cls \<Rightarrow> 'v literal multiset twl_clause" where
+"twl_clause C \<equiv> map_twl_clause (image_mset (\<lambda>L. the (lit_lookup C L))) (twl_cls C)"
+
+abbreviation clause_of_cls :: "'cls \<Rightarrow> 'v clause" where
+"clause_of_cls C \<equiv> clause (twl_clause C)"
+
+end
+
+locale abstract_clause_representation =
+  abstract_clause_representation_ops lit_lookup lit_keys twl_cls swap_lit
+    it_of_other_watched cls_ot_twl_list
+  for
+    lit_lookup :: "'cls \<Rightarrow> 'lit \<Rightarrow> 'v literal option" and
+    lit_keys :: "'cls \<Rightarrow> 'lit multiset" and
+
+    twl_cls :: "'cls \<Rightarrow> 'lit multiset twl_clause" and
+    swap_lit :: "'cls \<Rightarrow> 'lit \<Rightarrow> 'lit \<Rightarrow> 'cls" and
+    it_of_other_watched :: "'cls \<Rightarrow> 'lit \<Rightarrow> 'lit option" and
+    cls_ot_twl_list :: "'v literal list twl_clause \<Rightarrow> 'cls" +
   assumes
-    clause_twl_cls:
-      "clause (twl_cls C) = mset_cls C" and
-    clss_update:
-      "i \<in>\<Down> Cs \<Longrightarrow> clss_cls (clss_update Cs i C) = (clss_cls Cs) (i := C)" and
+    distinct_lit_keys[simp]: "distinct_mset (lit_keys C)" and
+    get_all_it: "i \<in># keys C \<longleftrightarrow> lit_lookup C i \<noteq> None" and
     swap_lit:
-      "j \<in>\<down> C \<Longrightarrow> k \<in>\<down> C \<Longrightarrow>
-        twl_clause_to_mset (twl_cls (swap_lit C j k)) =
-        TWL_Clause
-          ({#C\<down>k#} + mset (remove1 (C\<down>j) (watched (twl_cls C))))
-          ({#C\<down>j#} + mset (remove1 (C\<down>k) (watched (twl_cls C))))"
+      "j \<in># watched (twl_cls C) \<Longrightarrow> k \<in># unwatched (twl_cls C) \<Longrightarrow>
+        twl_cls (swap_lit C j k) =
+          TWL_Clause
+            ({#k#} + remove1_mset j (watched (twl_cls C)))
+            ({#j#} + remove1_mset k (unwatched (twl_cls C)))" and
+
+    it_of_other_watched:
+      "lit_lookup C j \<noteq> None \<Longrightarrow> it_of_other_watched C j = Some k \<Longrightarrow>
+         lit_lookup C k \<noteq> None \<and> k \<in># remove1_mset j (watched (twl_cls C))" and
+
+    twl_cls_valid:
+      "keys C = clause (twl_cls C)" and
+
+    cls_ot_twl_list:
+      "distinct (watched D @ unwatched D) \<Longrightarrow>
+        twl_clause (cls_ot_twl_list D) = map_twl_clause mset D"
 begin
 
 end
 
+locale abstract_clauses_representation =
+  fixes
+    cls_lookup :: "'clss \<Rightarrow> 'cls_it \<Rightarrow> 'cls option" and
+    cls_keys :: "'clss \<Rightarrow> 'cls_it multiset" and
+    clss_update :: "'clss \<Rightarrow> 'cls_it \<Rightarrow> 'cls \<Rightarrow> 'clss" and
+    add_cls :: "'clss \<Rightarrow> 'cls \<Rightarrow> 'clss \<times> 'cls_it"
+  assumes
+    cls_keys_distinct[simp]: "distinct_mset (cls_keys Cs)" and
+    cls_keys: "i \<in># cls_keys Cs \<longleftrightarrow> cls_lookup Cs i \<noteq> None" and
+    clss_update:
+      "cls_lookup Cs i \<noteq> None \<Longrightarrow> cls_lookup (clss_update Cs i C) = (cls_lookup Cs) (i := Some C)"
+      and
+    add_cls:
+      "add_cls Cs C = (Cs', i) \<Longrightarrow> cls_lookup Cs' = (cls_lookup Cs) (i := Some C)"  and
+    add_cls_new_keys:
+      "add_cls Cs C = (Cs', i) \<Longrightarrow> i \<notin># cls_keys Cs"
+begin
+
+lemma add_cls_new_key:
+  "add_cls Cs C = (Cs', i) \<Longrightarrow> i \<in># cls_keys Cs'"
+  unfolding cls_keys by (simp add: add_cls)
+
+abbreviation raw_clss :: "'clss \<Rightarrow> 'cls multiset" where
+"raw_clss Cs \<equiv> image_mset (\<lambda>L. the (cls_lookup Cs L)) (cls_keys Cs)"
+
+lemma cls_keys_clss_update[simp]:
+  "cls_lookup Cs i \<noteq> None \<Longrightarrow> cls_keys (clss_update Cs i E) = cls_keys Cs"
+  by (rule distinct_set_mset_eq) (auto simp: cls_keys clss_update split: if_splits)
+
+end
+
+locale abstract_clause_clauses_representation =
+  abstract_clause_representation lit_lookup lit_keys twl_cls swap_lit
+    it_of_other_watched cls_ot_twl_list +
+  abstract_clauses_representation cls_lookup cls_keys clss_update add_cls
+  for
+    lit_lookup :: "'cls \<Rightarrow> 'lit \<Rightarrow> 'v literal option" and
+    lit_keys :: "'cls \<Rightarrow> 'lit multiset" and
+
+    twl_cls :: "'cls \<Rightarrow> 'lit multiset twl_clause" and
+    swap_lit :: "'cls \<Rightarrow> 'lit \<Rightarrow> 'lit \<Rightarrow> 'cls" and
+    it_of_other_watched :: "'cls \<Rightarrow> 'lit \<Rightarrow> 'lit option" and
+
+    cls_ot_twl_list :: "'v literal list twl_clause \<Rightarrow> 'cls" and
+    cls_lookup :: "'clss \<Rightarrow> 'cls_it \<Rightarrow> 'cls option" and
+    cls_keys :: "'clss \<Rightarrow> 'cls_it multiset" and
+    clss_update :: "'clss \<Rightarrow> 'cls_it \<Rightarrow> 'cls \<Rightarrow> 'clss" and
+    add_cls :: "'clss \<Rightarrow> 'cls \<Rightarrow> 'clss \<times> 'cls_it"
+begin
+
+definition clauses_of_clss :: "'clss \<Rightarrow> 'v literal multiset multiset" where
+"clauses_of_clss N \<equiv> image_mset clause_of_cls (raw_clss N)"
+
+text \<open>The following abbreviation are useful to write shorter formula. Kill?\<close>
+definition the_lit_lookup :: "'cls \<Rightarrow> 'lit \<Rightarrow> 'v literal" (infix "\<down>" 49) where
+"C \<down> a \<equiv> the (lit_lookup C a)"
+
+definition the_cls_lookup :: "'clss \<Rightarrow> 'cls_it \<Rightarrow> 'cls" (infix "\<Down>" 49) where
+"C \<Down> a \<equiv> the (cls_lookup C a)"
+
+definition valid_lit_lookup :: "'lit \<Rightarrow> 'cls \<Rightarrow> bool" (infix "\<in>\<down>" 49) where
+"a \<in>\<down> Cs \<equiv> lit_lookup Cs a \<noteq> None"
+
+definition valid_cls_lookup :: "'cls_it \<Rightarrow> 'clss \<Rightarrow> bool" (infix "\<in>\<Down>" 49) where
+"a \<in>\<Down> Cs \<equiv> cls_lookup Cs a \<noteq> None"
+
+end
+
 locale abs_state\<^sub>W_clss_twl_ops =
-  raw_clss_with_update
-    get_lit mset_cls get_cls mset_clss
-    twl_cls clss_update swap_lit
+  abstract_clause_clauses_representation
+    lit_lookup lit_keys twl_cls swap_lit
+    it_of_other_watched cls_ot_twl_list
+
+    cls_lookup cls_keys clss_update add_cls
     +
   raw_cls mset_ccls
   for
     \<comment> \<open>Clause:\<close>
-    get_lit :: "'cls \<Rightarrow> 'lit \<Rightarrow> 'v literal option" and
-    mset_cls :: "'cls \<Rightarrow> 'v clause" and
+    lit_lookup :: "'cls \<Rightarrow> 'lit \<Rightarrow> 'v literal option" and
+    lit_keys :: "'cls \<Rightarrow> 'lit multiset" and
 
-    \<comment> \<open>Multiset of Clauses:\<close>
-    get_cls :: "'clss \<Rightarrow> 'cls_it \<Rightarrow> 'cls option" and
-    mset_clss:: "'clss \<Rightarrow> 'cls multiset" and
-
-    twl_cls :: "'cls \<Rightarrow> 'v literal list twl_clause" and
-    clss_update :: "'clss \<Rightarrow> 'cls_it \<Rightarrow> 'cls \<Rightarrow> 'clss" and
+    twl_cls :: "'cls \<Rightarrow> 'lit multiset twl_clause" and
     swap_lit :: "'cls \<Rightarrow> 'lit \<Rightarrow> 'lit \<Rightarrow> 'cls" and
+    it_of_other_watched :: "'cls \<Rightarrow> 'lit \<Rightarrow> 'lit option" and
+
+    \<comment> \<open>Clauses\<close>
+    cls_ot_twl_list :: "'v literal list twl_clause \<Rightarrow> 'cls" and
+    cls_lookup :: "'clss \<Rightarrow> 'cls_it \<Rightarrow> 'cls option" and
+    cls_keys :: "'clss \<Rightarrow> 'cls_it multiset" and
+    clss_update :: "'clss \<Rightarrow> 'cls_it \<Rightarrow> 'cls \<Rightarrow> 'clss" and
+    add_cls :: "'clss \<Rightarrow> 'cls \<Rightarrow> 'clss \<times> 'cls_it" and
 
     \<comment> \<open>Conflicting clause:\<close>
     mset_ccls :: "'ccls \<Rightarrow> 'v clause"
@@ -95,7 +198,7 @@ begin
 
 fun mmset_of_mlit :: "'clss \<Rightarrow> ('v, 'cls_it) ann_lit \<Rightarrow> ('v, 'v clause) ann_lit"
   where
-"mmset_of_mlit Cs (Propagated L C) = Propagated L (mset_cls (Cs \<Down> C))" |
+"mmset_of_mlit Cs (Propagated L C) = Propagated L (clause_of_cls (Cs \<Down> C))" |
 "mmset_of_mlit _ (Decided L) = Decided L"
 
 lemma lit_of_mmset_of_mlit[simp]:
@@ -110,52 +213,34 @@ lemma map_mmset_of_mlit_true_annots_true_cls[simp]:
   "map (mmset_of_mlit Cs) M' \<Turnstile>as C \<longleftrightarrow> M' \<Turnstile>as C"
   by (simp add: true_annots_true_cls lits_of_def)
 
-definition clauses_of_clss where
-"clauses_of_clss N \<equiv> image_mset mset_cls (mset_clss N)"
-
-notation cls_lit (infix "\<down>" 49)
-notation clss_cls (infix "\<Down>" 49)
-notation in_cls (infix "\<in>\<down>" 49)
-notation in_clss (infix "\<in>\<Down>" 49)
-
-lemma clauses_of_clss_met_cls:
-  "set_mset (clauses_of_clss Cs) = {mset_cls (Cs \<Down> i)|i. i \<in>\<Down> Cs}"
-  unfolding clauses_of_clss_def clss_cls_def in_clss_def
-  apply (auto dest!: in_mset_clss_exists_preimage)
-  by (metis option.sel)
-
-lemma finite_mset_cls: "finite {mset_cls (Cs \<Down> i)|i. i \<in>\<Down> Cs}"
-  unfolding clauses_of_clss_met_cls[symmetric] by auto
-
-lemma clauses_of_clss_mset_met_cls:
-  assumes "distinct_mset (clauses_of_clss Cs)"
-  shows "clauses_of_clss Cs = mset_set {mset_cls (Cs \<Down> i)|i. i \<in>\<Down> Cs}"
-  using clauses_of_clss_met_cls distinct_mset_set_mset_ident[OF assms] by force
-
 end
 
 
 locale abs_state\<^sub>W_twl_ops =
   abs_state\<^sub>W_clss_twl_ops
     \<comment> \<open>functions for clauses: \<close>
-    cls_lit mset_cls
-    clss_cls mset_clss
-    twl_cls clss_update swap_lit
+    lit_lookup lit_keys twl_cls swap_lit
+    it_of_other_watched cls_ot_twl_list
+
+    cls_lookup cls_keys clss_update add_cls
 
     \<comment> \<open>functions for the conflicting clause:\<close>
     mset_ccls
   for
     \<comment> \<open>Clause:\<close>
-    cls_lit :: "'cls \<Rightarrow> 'lit \<Rightarrow> 'v literal option" and
-    mset_cls :: "'cls \<Rightarrow> 'v clause" and
+    lit_lookup :: "'cls \<Rightarrow> 'lit \<Rightarrow> 'v literal option" and
+    lit_keys :: "'cls \<Rightarrow> 'lit multiset" and
 
-    \<comment> \<open>Multiset of Clauses:\<close>
-    clss_cls :: "'clss \<Rightarrow> 'cls_it \<Rightarrow> 'cls option" and
-    mset_clss:: "'clss \<Rightarrow> 'cls multiset" and
-
-    twl_cls :: "'cls \<Rightarrow> 'v literal list twl_clause" and
-    clss_update :: "'clss \<Rightarrow> 'cls_it \<Rightarrow> 'cls \<Rightarrow> 'clss" and
+    twl_cls :: "'cls \<Rightarrow> 'lit multiset twl_clause" and
     swap_lit :: "'cls \<Rightarrow> 'lit \<Rightarrow> 'lit \<Rightarrow> 'cls" and
+    it_of_other_watched :: "'cls \<Rightarrow> 'lit \<Rightarrow> 'lit option" and
+
+    \<comment> \<open>Clauses\<close>
+    cls_ot_twl_list :: "'v literal list twl_clause \<Rightarrow> 'cls" and
+    cls_lookup :: "'clss \<Rightarrow> 'cls_it \<Rightarrow> 'cls option" and
+    cls_keys :: "'clss \<Rightarrow> 'cls_it multiset" and
+    clss_update :: "'clss \<Rightarrow> 'cls_it \<Rightarrow> 'cls \<Rightarrow> 'clss" and
+    add_cls :: "'clss \<Rightarrow> 'cls \<Rightarrow> 'clss \<times> 'cls_it" and
 
     \<comment> \<open>Conflicting clause:\<close>
     mset_ccls :: "'ccls \<Rightarrow> 'v clause" +
@@ -217,17 +302,37 @@ fun valid_annotation :: "'st \<Rightarrow> ('a, 'cls_it) ann_lit \<Rightarrow> b
 end
 
 
+lemma image_mset_if_eq_index:
+  "{#if x = i then P x else Q x. x \<in># M#} =
+  {#Q x. x \<in># removeAll_mset i M#} + replicate_mset (count M i) (P i)" (is "?M M = _")
+proof -
+  have M: "M = filter_mset (op = i) M + filter_mset (op \<noteq> i) M"
+    by (auto simp: multiset_eq_iff)
+  have "?M M = ?M (filter_mset (op = i) M) + ?M (filter_mset (op \<noteq> i) M)"
+     by (subst M) simp
+  moreover have "?M (filter_mset (op = i) M) = replicate_mset (count M i) (P i)"
+    by (simp add: filter_mset_eq)
+  moreover have "?M (filter_mset (op \<noteq> i) M) = {#Q x. x \<in># removeAll_mset i M#}"
+    apply (subst removeAll_mset_filter_mset)
+    apply (rule image_mset_cong2)
+    by auto
+  ultimately show ?thesis
+    by (auto simp: ac_simps not_in_iff)
+qed
+
 locale abs_state\<^sub>W_twl =
   abs_state\<^sub>W_twl_ops
-    cls_lit mset_cls
-    clss_cls mset_clss
-    twl_cls clss_update swap_lit
+    \<comment> \<open>functions for clauses: \<close>
+    lit_lookup lit_keys twl_cls swap_lit
+    it_of_other_watched cls_ot_twl_list
+
+    cls_lookup cls_keys clss_update add_cls
 
     \<comment> \<open>functions for the conflicting clause:\<close>
     mset_ccls
-    
+
     find_undef_in_unwatched
-    
+
     conc_trail hd_raw_conc_trail prop_queue raw_clauses conc_backtrack_lvl raw_conc_conflicting
 
     conc_learned_clss
@@ -246,16 +351,19 @@ locale abs_state\<^sub>W_twl =
 
   for
     \<comment> \<open>Clause:\<close>
-    cls_lit :: "'cls \<Rightarrow> 'lit \<Rightarrow> 'v literal option" and
-    mset_cls :: "'cls \<Rightarrow> 'v clause" and
+    lit_lookup :: "'cls \<Rightarrow> 'lit \<Rightarrow> 'v literal option" and
+    lit_keys :: "'cls \<Rightarrow> 'lit multiset" and
 
-    \<comment> \<open>Multiset of Clauses:\<close>
-    clss_cls :: "'clss \<Rightarrow> 'cls_it \<Rightarrow> 'cls option" and
-    mset_clss:: "'clss \<Rightarrow> 'cls multiset" and
-
-    twl_cls :: "'cls \<Rightarrow> 'v literal list twl_clause" and
-    clss_update :: "'clss \<Rightarrow> 'cls_it \<Rightarrow> 'cls \<Rightarrow> 'clss" and
+    twl_cls :: "'cls \<Rightarrow> 'lit multiset twl_clause" and
     swap_lit :: "'cls \<Rightarrow> 'lit \<Rightarrow> 'lit \<Rightarrow> 'cls" and
+    it_of_other_watched :: "'cls \<Rightarrow> 'lit \<Rightarrow> 'lit option" and
+
+    \<comment> \<open>Clauses\<close>
+    cls_ot_twl_list :: "'v literal list twl_clause \<Rightarrow> 'cls" and
+    cls_lookup :: "'clss \<Rightarrow> 'cls_it \<Rightarrow> 'cls option" and
+    cls_keys :: "'clss \<Rightarrow> 'cls_it multiset" and
+    clss_update :: "'clss \<Rightarrow> 'cls_it \<Rightarrow> 'cls \<Rightarrow> 'clss" and
+    add_cls :: "'clss \<Rightarrow> 'cls \<Rightarrow> 'clss \<times> 'cls_it" and
 
     \<comment> \<open>Conflicting clause:\<close>
     mset_ccls :: "'ccls \<Rightarrow> 'v clause" and
@@ -322,129 +430,110 @@ locale abs_state\<^sub>W_twl =
       "get_undecided_lit T = None \<longleftrightarrow>
          (\<forall>L'. atm_of L' \<in> atms_of_mm (conc_clauses T) \<longrightarrow> \<not>undefined_lit (conc_trail T) L')" and
     get_clause_watched_by:
-      "i \<in> set (get_clause_watched_by T K) \<longleftrightarrow> K \<in> set (watched (twl_cls (raw_clauses T \<Down> i)))" and
+      "i \<in> set (get_clause_watched_by T K) \<longleftrightarrow> K \<in># watched (twl_clause (raw_clauses T \<Down> i))" and
     get_clause_watched_by_distinct:
       "distinct (get_clause_watched_by T K)" and
+
     update_clause:
       "i \<in>\<Down> raw_clauses S \<Longrightarrow>
-        clss_cls (raw_clauses (update_clause S i E)) = (clss_cls (raw_clauses S)) (i := Some E)" and
+        raw_clauses (update_clause S i E) = clss_update (raw_clauses S) i E" and
     update_clause_state:
       "i \<in>\<Down> raw_clauses S \<Longrightarrow> state S = (M, N, U, k, C) \<Longrightarrow>
         state (update_clause S i E) = (M, conc_init_clss S, conc_learned_clss S, k, C)" and
-        
+
     find_undef_in_unwatched_Some:
       "find_undef_in_unwatched S E = Some j \<Longrightarrow> j \<in>\<down> E \<and> undefined_lit (full_trail S) (E\<down>j) \<and>
-        (E\<down>j) \<in> set (unwatched (twl_cls E))" and
+        (E\<down>j) \<in># unwatched (twl_clause E)" and
     find_undef_in_unwatched_None:
-      "find_undef_in_unwatched S E = None \<longleftrightarrow> 
-        (\<forall>j. j \<in>\<down> E \<longrightarrow> (E\<down>j) \<in> set (unwatched (twl_cls E)) \<longrightarrow>
+      "find_undef_in_unwatched S E = None \<longleftrightarrow>
+        (\<forall>j. j \<in>\<down> E \<longrightarrow> (E\<down>j) \<in># unwatched (twl_clause E) \<longrightarrow>
            \<not>undefined_lit (full_trail S) (E\<down>j))"
 begin
 
-lemma
+lemma conc_clauses_update_clause:
   assumes
-    "i \<in>\<Down> raw_clauses S" and [simp]: "distinct_mset (clauses_of_clss (raw_clauses S))" and
-    [simp]: "mset_cls (raw_clauses S \<Down> i) = mset_cls E"
+    i: "i \<in>\<Down> raw_clauses S"
   shows
     "conc_clauses (update_clause S i E) =
-       remove1_mset (mset_cls (raw_clauses S \<Down> i)) (conc_clauses S) + {#mset_cls E#}"
+       remove1_mset (clause_of_cls (raw_clauses S \<Down> i)) (conc_clauses S) + {#clause_of_cls E#}"
      (is "?conc = ?r")
-proof -
-  have H: "clauses_of_clss (raw_clauses S) =
-    mset_set {mset_cls (raw_clauses S \<Down> i) |i. i \<in>\<Down> raw_clauses S}"
-    using clauses_of_clss_mset_met_cls by auto
-  then have dist': "distinct_mset ?r"
-    unfolding conc_clauses_def clauses_of_clss_mset_met_cls[OF assms(2)] 
-    using assms(2) H  distinct_mem_diff_mset distinct_mset_single_add by fastforce
-    
-  have T: "remove1_mset (mset_cls E) (mset_set {mset_cls (raw_clauses S \<Down> i) |i. i \<in>\<Down> raw_clauses S})
-    + {#mset_cls E#} = mset_set {mset_cls (raw_clauses S \<Down> i) |i. i \<in>\<Down> raw_clauses S}"
-proof -
-  have "mset_cls E \<in> {mset_cls (raw_clauses S \<Down> c) |c. c \<in>\<Down> raw_clauses S}"
-    using assms(1) by force (* 2 ms *)
-  then show ?thesis
-    by (metis (no_types) H clauses_of_clss_met_cls insert_DiffM union_commute) (* 696 ms *)
-qed
-  then have [simp]:
-    "remove1_mset (mset_cls E) (image_mset mset_cls (mset_clss (raw_clauses S))) + {#mset_cls E#} =
-      image_mset mset_cls (mset_clss (raw_clauses S))"
-    using H unfolding clauses_of_clss_def by auto
+proof-
+  have XX: "\<And>x. clause_of_cls (the (if x = i then Some E else cls_lookup (raw_clauses S) x)) =
+    (if x = i then clause_of_cls E else clause_of_cls (the (cls_lookup (raw_clauses S) x)))"
+     by (auto simp: update_clause[OF i] clss_update split: if_splits)
+  have YY: "remove1_mset (clause_of_cls (raw_clauses S \<Down> i))
+    {#clause_of_cls (the (cls_lookup (raw_clauses S) x)). x \<in># cls_keys (raw_clauses S)#} =
+    {#clause_of_cls (the (cls_lookup (raw_clauses S) x)).
+       x \<in># remove1_mset i (cls_keys (raw_clauses S))#}"
+     apply (subst subseteq_image_mset_minus)
+     using i by (auto simp: valid_cls_lookup_def cls_keys the_cls_lookup_def)
+
+  have c: "count (cls_keys (raw_clauses S)) i = 1"
+    by (meson cls_keys cls_keys_distinct distinct_mset_def i valid_cls_lookup_def)
+  then have [simp]: "replicate_mset (count (cls_keys (raw_clauses S)) i) (clause_of_cls E) =
+    {#clause_of_cls E#}"
+    by simp
   show ?thesis
-    unfolding conc_clauses_def clauses_of_clss_mset_met_cls[OF assms(2)]
-    clauses_of_clss_def
-    using update_clause 
-    apply (auto simp add: update_clause assms(1))
-    apply (subst (2) clauses_of_clss_mset_met_cls[unfolded clauses_of_clss_def])
-      using dist' unfolding conc_clauses_def clauses_of_clss_mset_met_cls[OF assms(2)]
-    clauses_of_clss_def apply (auto simp:) 
-    defer
-      defer
-      
-    using clauses_of_clss_mset_met_cls unfolding clauses_of_clss_def
-    
-    unfolding conc_clauses_def clauses_of_clss_mset_met_cls[OF ]
-    
+     using i unfolding conc_clauses_def clauses_of_clss_def valid_cls_lookup_def
+     by (auto simp: update_clause[OF i] clss_update XX YY image_mset_if_eq_index
+       distinct_mset_remove1_All)
+qed
+
 end
 
 locale abs_conflict_driven_clause_learning\<^sub>W_clss =
-  twl_state\<^sub>W_clss
-    \<comment> \<open>functions for clauses: \<close>
-    cls_lit in_cls mset_cls
-    clss_cls in_clss mset_clss
+  abs_state\<^sub>W_twl
+     \<comment> \<open>functions for clauses: \<close>
+    lit_lookup lit_keys twl_cls swap_lit
+    it_of_other_watched cls_ot_twl_list
+
+    cls_lookup cls_keys clss_update add_cls
 
     \<comment> \<open>functions for the conflicting clause:\<close>
     mset_ccls
 
-    twl_cls clss_update swap_lit  exists_in_unwatched
-    \<comment> \<open>functions about the state:\<close>
-      \<comment> \<open>getter:\<close>
-    conc_trail hd_raw_conc_trail raw_clauses conc_backtrack_lvl
-    raw_conc_conflicting conc_learned_clss
-      \<comment> \<open>setter:\<close>
-    cons_conc_trail tl_conc_trail add_conc_confl_to_learned_cls conc_remove_cls
-    update_conc_backtrack_lvl
-    mark_conflicting reduce_conc_trail_to resolve_conflicting
+    find_undef_in_unwatched
 
-      \<comment> \<open>Some specific states:\<close>
-    conc_init_state
-    restart_state
+    conc_trail hd_raw_conc_trail prop_queue raw_clauses conc_backtrack_lvl raw_conc_conflicting
 
-      -- \<open>Additional functions:\<close>
-        -- \<open>Propagate queue\<close>
-    prop_queue
-    cons_prop_queue
-    hd_prop_queue_to_trail
-    prop_queue_to_trail
+    conc_learned_clss
 
-        -- \<open>Not decided literals\<close>
-    get_undecided_lit
+    cons_conc_trail tl_conc_trail reduce_conc_trail_to
 
-        -- \<open>Watched clauses:\<close>
-    get_clause_watched_by
+    cons_prop_queue hd_prop_queue_to_trail prop_queue_to_trail
 
-    update_clause
+    add_conc_confl_to_learned_cls conc_remove_cls
+
+    update_conc_backtrack_lvl mark_conflicting resolve_conflicting
+
+    get_undecided_lit get_clause_watched_by update_clause
+
+    conc_init_state restart_state
 
   for
     \<comment> \<open>Clause:\<close>
-    cls_lit :: "'cls \<Rightarrow> 'lit \<Rightarrow> 'v literal" and
-    in_cls :: "'lit \<Rightarrow> 'cls \<Rightarrow> bool" and
-    mset_cls :: "'cls \<Rightarrow> 'v clause" and
+    lit_lookup :: "'cls \<Rightarrow> 'lit \<Rightarrow> 'v literal option" and
+    lit_keys :: "'cls \<Rightarrow> 'lit multiset" and
 
-    \<comment> \<open>Multiset of Clauses:\<close>
-    clss_cls :: "'clss \<Rightarrow> 'cls_it \<Rightarrow> 'cls" and
-    in_clss :: "'cls_it \<Rightarrow> 'clss \<Rightarrow> bool" and
-    mset_clss:: "'clss \<Rightarrow> 'cls multiset" and
+    twl_cls :: "'cls \<Rightarrow> 'lit multiset twl_clause" and
+    swap_lit :: "'cls \<Rightarrow> 'lit \<Rightarrow> 'lit \<Rightarrow> 'cls" and
+    it_of_other_watched :: "'cls \<Rightarrow> 'lit \<Rightarrow> 'lit option" and
+
+    \<comment> \<open>Clauses\<close>
+    cls_ot_twl_list :: "'v literal list twl_clause \<Rightarrow> 'cls" and
+    cls_lookup :: "'clss \<Rightarrow> 'cls_it \<Rightarrow> 'cls option" and
+    cls_keys :: "'clss \<Rightarrow> 'cls_it multiset" and
+    clss_update :: "'clss \<Rightarrow> 'cls_it \<Rightarrow> 'cls \<Rightarrow> 'clss" and
+    add_cls :: "'clss \<Rightarrow> 'cls \<Rightarrow> 'clss \<times> 'cls_it" and
 
     \<comment> \<open>Conflicting clause:\<close>
     mset_ccls :: "'ccls \<Rightarrow> 'v clause" and
 
-    \<comment> \<open>2 watched literals conversion:\<close>
-    twl_cls :: "'cls \<Rightarrow> 'v literal list twl_clause" and
-    clss_update :: "'clss \<Rightarrow> 'cls_it \<Rightarrow> 'cls \<Rightarrow> 'clss" and
-    swap_lit :: "'cls \<Rightarrow> 'lit \<Rightarrow> 'lit \<Rightarrow> 'cls" and
-    exists_in_unwatched :: "('lit \<Rightarrow> bool) \<Rightarrow> 'cls \<Rightarrow> 'lit option" and
+    find_undef_in_unwatched :: "'st \<Rightarrow> 'cls \<Rightarrow> 'lit option" and
+
     conc_trail :: "'st \<Rightarrow> ('v, 'v clause) ann_lits" and
     hd_raw_conc_trail :: "'st \<Rightarrow> ('v, 'cls_it) ann_lit" and
+    prop_queue :: "'st \<Rightarrow> ('v, 'v clause) ann_lits" and
     raw_clauses :: "'st \<Rightarrow> 'clss" and
     conc_backtrack_lvl :: "'st \<Rightarrow> nat" and
     raw_conc_conflicting :: "'st \<Rightarrow> 'ccls option" and
@@ -453,25 +542,27 @@ locale abs_conflict_driven_clause_learning\<^sub>W_clss =
 
     cons_conc_trail :: "('v, 'cls_it) ann_lit \<Rightarrow> 'st \<Rightarrow> 'st" and
     tl_conc_trail :: "'st \<Rightarrow> 'st" and
-    add_conc_confl_to_learned_cls :: "'st \<Rightarrow> 'st" and
-    conc_remove_cls :: "'cls \<Rightarrow> 'st \<Rightarrow> 'st" and
-    update_conc_backtrack_lvl :: "nat \<Rightarrow> 'st \<Rightarrow> 'st" and
-    mark_conflicting :: "'cls_it \<Rightarrow> 'st \<Rightarrow> 'st" and
     reduce_conc_trail_to :: "('v, 'v clause) ann_lits \<Rightarrow> 'st \<Rightarrow> 'st" and
-    resolve_conflicting :: "'v literal \<Rightarrow> 'cls \<Rightarrow> 'st \<Rightarrow> 'st" and
 
-    conc_init_state :: "'clss \<Rightarrow> 'st" and
-    restart_state :: "'st \<Rightarrow> 'st" and
-
-    prop_queue :: "'st \<Rightarrow> ('v, 'v clause) ann_lits" and
     cons_prop_queue :: "('v, 'cls_it) ann_lit \<Rightarrow> 'st \<Rightarrow> 'st" and
     hd_prop_queue_to_trail :: "'st \<Rightarrow> 'st" and
     prop_queue_to_trail :: "'st \<Rightarrow> 'st" and
 
+    add_conc_confl_to_learned_cls :: "'st \<Rightarrow> 'st" and
+    conc_remove_cls :: "'cls \<Rightarrow> 'st \<Rightarrow> 'st" and
+
+    update_conc_backtrack_lvl :: "nat \<Rightarrow> 'st \<Rightarrow> 'st" and
+
+    mark_conflicting :: "'cls_it \<Rightarrow> 'st \<Rightarrow> 'st" and
+    resolve_conflicting :: "'v literal \<Rightarrow> 'cls \<Rightarrow> 'st \<Rightarrow> 'st" and
+
     get_undecided_lit :: "'st \<Rightarrow> 'v literal option" and
     get_clause_watched_by :: "'st \<Rightarrow> 'v literal \<Rightarrow> 'cls_it list" and
-    update_clause :: "'st \<Rightarrow> 'cls_it \<Rightarrow> 'cls \<Rightarrow> 'st"
-begin
+    update_clause :: "'st \<Rightarrow> 'cls_it \<Rightarrow> 'cls \<Rightarrow> 'st" and
+
+    conc_init_state :: "'clss \<Rightarrow> 'st" and
+    restart_state :: "'st \<Rightarrow> 'st"
+begin(*
 
 fun other_watched_lit  where
 "other_watched_lit S i L =
@@ -491,7 +582,7 @@ fun update_clause where
          (\<lambda>j. undefined_lit (conc_trail S) ((raw_clauses S \<Down> i) \<down> j)) (raw_clauses S \<Down> i) of
          None \<Rightarrow> mark_conflicting i S
        | Some _ \<Rightarrow> S)
-     )"
+     )" *)
 
 end
 
